feat: Add UTF8 and Single Value

TestModels/SimpleTypes/SimpleString/src/SimpleStringImpl.dfy
@@ -10,10 +10,27 @@ module SimpleStringImpl refines AbstractSimpleTypesStringOperations  {
    predicate GetStringEnsuresPublicly(input: GetStringInput, output: Result<GetStringOutput, Error>) {
     true
    }
+   predicate GetStringSingleValueEnsuresPublicly(input: GetStringInput, output: Result<GetStringOutput, Error>) {
+    true
+   }
+   predicate GetStringUTF8EnsuresPublicly(input: GetStringInput, output: Result<GetStringOutput, Error>) {
+    true
+   }
  method GetString ( config: InternalConfig,  input: GetStringInput )
  returns (output: Result<GetStringOutput, Error>) {
+    var res := GetStringOutput(value := input.value);
+    return Success(res);
+ }
+ method GetStringSingleValue ( config: InternalConfig,  input: GetStringInput )
+ returns (output: Result<GetStringOutput, Error>) {
     expect input.value.Some?;
-    expect input.value.value == "TEST_SIMPLE_STRING_VALUE"; // This is done so as to assert that polymorph layer is doing one way conversion right as well.
+    expect input.value.value == "TEST_SIMPLE_STRING_SINGLE_VALUE"; // This is done so as to assert that polymorph layer is doing one way conversion right as well.
+    var res := GetStringOutput(value := input.value);
+    return Success(res);
+ }
+ method GetStringUTF8 ( config: InternalConfig,  input: GetStringInput )
+ returns (output: Result<GetStringOutput, Error>) {
+    expect input.value.Some?;
     var res := GetStringOutput(value := input.value);
     return Success(res);
  }
