TestModels/SimpleTypes/SimpleString/test/SimpleStringImplTest.dfy
@@ -7,6 +7,8 @@ module  SimpleStringImplTest {
     method{:test} GetString(){
         var client :- expect SimpleString.SimpleString();
         TestGetString(client);
+        TestGetStringSingleValue(client);
+        TestGetStringUTF8(client);
     }
 
     method TestGetString(client: ISimpleTypesStringClient)
@@ -16,6 +18,26 @@ module  SimpleStringImplTest {
     {
         var ret :- expect client.GetString(SimpleString.Types.GetStringInput(value:= Some("TEST_SIMPLE_STRING_VALUE")));
         expect ret.value.UnwrapOr("") == "TEST_SIMPLE_STRING_VALUE";
+        print ret;
+    }
+    method TestGetStringSingleValue(client: ISimpleTypesStringClient)
+      requires client.ValidState()
+      modifies client.Modifies
+      ensures client.ValidState()
+    {
+        var ret :- expect client.GetStringSingleValue(SimpleString.Types.GetStringInput(value:= Some("TEST_SIMPLE_STRING_SINGLE_VALUE")));
+        expect ret.value.UnwrapOr("") == "TEST_SIMPLE_STRING_SINGLE_VALUE";
+        print ret;
+    }
+    method TestGetStringUTF8(client: ISimpleTypesStringClient)
+      requires client.ValidState()
+      modifies client.Modifies
+      ensures client.ValidState()
+    {
+        // a = TEST_SIMPLE_STRING_UTF8_VALUE
+        var a := "\u0054\u0045\u0053\u0054\u005f\u0053\u0049\u004d\u0050\u004c\u0045\u005f\u0053\u0054\u0052\u0049\u004e\u0047\u005f\u0055\u0054\u0046\u0038\u005f\u0056\u0041\u004c\u0055\u0045";
+        var ret :- expect client.GetStringUTF8(SimpleString.Types.GetStringInput(value:= Some(a)));
+        expect ret.value.UnwrapOr("") == a;
         print ret;
     }
 }
