TestModels/SimpleTypes/SimpleString/Model/SimpleString.smithy
@@ -7,13 +7,23 @@ namespace simple.types.string
 service SimpleTypesString {
   version: "2021-11-01",
   resources: [],
-  operations: [ GetString ],
+  operations: [ GetString, GetStringSingleValue, GetStringUTF8 ],
   errors: [],
 }
 
 structure SimpleStringConfig {}
 
 operation GetString {
+  input: GetStringInput,
+  output: GetStringOutput,
+}
+
+operation GetStringSingleValue {
+  input: GetStringInput,
+  output: GetStringOutput,
+}
+
+operation GetStringUTF8 {
   input: GetStringInput,
   output: GetStringOutput,
 }
